code/experimental/SPARKLE/dist/test_implementation_1.c
@@ -19,64 +19,13 @@ void sparkle_modified1 ( uint32_t * state , int nb , int ns )
 
 	Hacl_Impl_Sparkle_add2(nb, i, state);
 	Hacl_Impl_Sparkle_arx_n(nb, state);
-
-
-	uint32_t tx = (uint32_t)0U;
-  	uint32_t ty = (uint32_t)0U;
-
-
-  	Hacl_Impl_Sparkle_xor(nb, state, &tx, &ty);
-	tmpx = (tx << (uint32_t)16U | tx >> (uint32_t)16U) ^ (tx & (uint32_t)0xffffU);
-	tmpy = (ty << (uint32_t)16U | ty >> (uint32_t)16U) ^ (ty & (uint32_t)0xffffU);
-	Hacl_Impl_Sparkle_xor_x(nb, state, tmpy, tmpx);
-
-
-
-	// uint32_t tx = (uint32_t)0U;
-	// uint32_t ty = (uint32_t)0U;
-	// Hacl_Impl_Sparkle_xor(n, b, &tx, &ty);
-	// uint32_t uu____0 = tx;
-	// uint32_t
-	// 	ltx = (uu____0 << (uint32_t)16U | uu____0 >> (uint32_t)16U) ^ (uu____0 & (uint32_t)0xffffU);
+	Hacl_Impl_Sparkle_l(nb, state); 
 	
-	// uint32_t uu____1 = ty;
-	// uint32_t
-	//   lty = (uu____1 << (uint32_t)16U | uu____1 >> (uint32_t)16U) ^ (uu____1 & (uint32_t)0xffffU);
-	// Hacl_Impl_Sparkle_xor_x(n, b, lty, ltx);
+	state[2] = state[8];
+	state[3] = state[9];
+	state[0] = state[10];
+	state[1] = state[11];
 
-
-
-  	x0 = state [0];
-	y0 = state [1];
-
-
-
-	// // does not influence
-	// state [0] = state [0] ^ tmpy;
-	// state [2] = state [2] ^ tmpy;
-
-	// // does not influence
-	// state[1] = state[1] ^ tmpx;
-	// state[3] = state[3] ^ tmpx;
-
-
-	state [0] = state [6] ^ state [2];
-	state [6] = state [2] ^ tmpy;
-	state [1] = state [7] ^ state [3] ;
-	state [7] = state [3] ^ tmpx ;
-
-	
-	// state [2] = state [8] ^ state [4] ^ tmpy ;
-	// state [2] = state [4];
-	// state [8] = state [4];
-	// state [3] = state [9] ^ state [5] ^ tmpx ;
-	// state [3] = state [5] ^ tmpx;
-	// state [9] = state [5];
-
-	state [2] = state [4] ^ x0;
-	state [4] = x0 ^ tmpy;
-	state [3] = state [5] ^ y0;
-	state [5] = y0 ^ tmpx; 
 }
 
 
